comex

lunarlander_sl/comex.thy
@@ -246,8 +246,7 @@ inductive P_inv_ind :: "real \<Rightarrow> real \<Rightarrow> (real \<times> rea
   "P_inv_ind a b [] []"
 | " a = b \<longrightarrow> (
   (Waitinv\<^sub>t (gsb2gsrb(sb2gsb inv)) (\<lambda> d. d = 1) ({}, {}) 
-  @\<^sub>t Waitinv\<^sub>t (gsb2gsrb(sb2gsb inv)) (\<lambda>_. True) ({''P2C''}, {})
-  @\<^sub>t Outinv\<^sub>t (\<lambda>_. True) (srb2gsrb (\<lambda> s v. v = s X)) ''P2C'' 
+  @\<^sub>t WaitOutinv\<^sub>t (gsb2gsrb(sb2gsb inv)) (\<lambda>_. True) (srb2gsrb (\<lambda> s v. v = s X)) ({''P2C''}, {}) ''P2C''
   @\<^sub>t Ininv\<^sub>t (\<lambda>_. True) (srb2gsrb (\<lambda> s v. v = a')) ''C2P'' 
   @\<^sub>t Ininv\<^sub>t (\<lambda>_. True) (srb2gsrb (\<lambda> s v. v = b')) ''C2P'') tr1 
      \<and> P_inv_ind a' b' Fcs tr2) \<Longrightarrow> P_inv_ind a b ((a',b')#Fcs) (tr1@tr2)"
@@ -330,8 +329,7 @@ lemma P_inv_snoc:
 "P_inv_ind a b fcs tr1 \<Longrightarrow> 
   same_pair ((a,b)#fcs) \<longrightarrow> 
     (Waitinv\<^sub>t (gsb2gsrb(sb2gsb inv)) (\<lambda> d. d = 1)({}, {}) 
-  @\<^sub>t Waitinv\<^sub>t (gsb2gsrb(sb2gsb inv)) (\<lambda> _. True) ({''P2C''}, {}) 
-  @\<^sub>t out_inv_assn (\<lambda>_. True) (srb2gsrb (\<lambda> s v. v = s X)) ''P2C'' 
+  @\<^sub>t WaitOutinv\<^sub>t (gsb2gsrb(sb2gsb inv)) (\<lambda>_. True) (srb2gsrb (\<lambda> s v. v = s X)) ({''P2C''}, {}) ''P2C'' 
   @\<^sub>t in_inv_assn  (\<lambda>_. True) (srb2gsrb (\<lambda> s v. v = a')) ''C2P'' 
   @\<^sub>t in_inv_assn  (\<lambda>_. True) (srb2gsrb (\<lambda> s v. v = b')) ''C2P'') tr2
                    \<Longrightarrow> P_inv_ind a b (fcs@[(a',b')]) (tr1@tr2)"
@@ -364,48 +362,41 @@ apply(auto simp add: emp_assn_def)
 lemma P_inv_prop1:
   assumes "a=b"
   shows "P_inv_ind a b ((a',b')#list) = Waitinv\<^sub>t (gsb2gsrb(sb2gsb inv)) (\<lambda> d. d = 1) ({}, {}) 
-  @\<^sub>t Waitinv\<^sub>t (gsb2gsrb(sb2gsb inv)) (\<lambda>_. True) ({''P2C''}, {})
-  @\<^sub>t Outinv\<^sub>t (\<lambda>_. True) (srb2gsrb (\<lambda> s v. v = s X)) ''P2C'' 
+  @\<^sub>t WaitOutinv\<^sub>t (gsb2gsrb(sb2gsb inv)) (\<lambda>_. True) (srb2gsrb (\<lambda> s v. v = s X)) ({''P2C''}, {}) ''P2C'' 
   @\<^sub>t Ininv\<^sub>t (\<lambda>_. True) (srb2gsrb (\<lambda> s v. v = a')) ''C2P'' 
   @\<^sub>t Ininv\<^sub>t (\<lambda>_. True) (srb2gsrb (\<lambda> s v. v = b')) ''C2P'' @\<^sub>t P_inv_ind a' b' list"
   apply(rule ext)
   subgoal for tr
 proof-
   have 1:"P_inv_ind a b ((a',b')#list) tr \<Longrightarrow> \<exists> tr1 tr2. (Waitinv\<^sub>t (gsb2gsrb(sb2gsb inv)) (\<lambda> d. d = 1) ({}, {}) 
-  @\<^sub>t Waitinv\<^sub>t (gsb2gsrb(sb2gsb inv)) (\<lambda>_. True) ({''P2C''}, {})
-  @\<^sub>t Outinv\<^sub>t (\<lambda>_. True) (srb2gsrb (\<lambda> s v. v = s X)) ''P2C'' 
+  @\<^sub>t WaitOutinv\<^sub>t (gsb2gsrb(sb2gsb inv)) (\<lambda>_. True) (srb2gsrb (\<lambda> s v. v = s X)) ({''P2C''}, {}) ''P2C''
   @\<^sub>t Ininv\<^sub>t (\<lambda>_. True) (srb2gsrb (\<lambda> s v. v = a')) ''C2P'' 
   @\<^sub>t Ininv\<^sub>t (\<lambda>_. True) (srb2gsrb (\<lambda> s v. v = b')) ''C2P'') tr1 \<and> P_inv_ind a' b' list tr2 \<and> tr= tr1@tr2"
     apply(rule P_inv_ind.cases[of a b "(a', b') # list" tr])
     using assms by auto
   then have 2:"P_inv_ind a b ((a',b')#list) tr \<Longrightarrow> ((Waitinv\<^sub>t (gsb2gsrb(sb2gsb inv)) (\<lambda> d. d = 1) ({}, {}) 
-  @\<^sub>t Waitinv\<^sub>t (gsb2gsrb(sb2gsb inv)) (\<lambda>_. True) ({''P2C''}, {})
-  @\<^sub>t Outinv\<^sub>t (\<lambda>_. True) (srb2gsrb (\<lambda> s v. v = s X)) ''P2C'' 
+  @\<^sub>t WaitOutinv\<^sub>t (gsb2gsrb(sb2gsb inv)) (\<lambda>_. True) (srb2gsrb (\<lambda> s v. v = s X)) ({''P2C''}, {}) ''P2C''
   @\<^sub>t Ininv\<^sub>t (\<lambda>_. True) (srb2gsrb (\<lambda> s v. v = a')) ''C2P'' 
   @\<^sub>t Ininv\<^sub>t (\<lambda>_. True) (srb2gsrb (\<lambda> s v. v = b')) ''C2P'') @\<^sub>t P_inv_ind a' b' list) tr"
     by(auto simp add:join_assn_def)
   have 3:"((Waitinv\<^sub>t (gsb2gsrb(sb2gsb inv)) (\<lambda> d. d = 1) ({}, {}) 
-  @\<^sub>t Waitinv\<^sub>t (gsb2gsrb(sb2gsb inv)) (\<lambda>_. True) ({''P2C''}, {})
-  @\<^sub>t Outinv\<^sub>t (\<lambda>_. True) (srb2gsrb (\<lambda> s v. v = s X)) ''P2C'' 
+  @\<^sub>t WaitOutinv\<^sub>t (gsb2gsrb(sb2gsb inv)) (\<lambda>_. True) (srb2gsrb (\<lambda> s v. v = s X)) ({''P2C''}, {}) ''P2C''
   @\<^sub>t Ininv\<^sub>t (\<lambda>_. True) (srb2gsrb (\<lambda> s v. v = a')) ''C2P'' 
   @\<^sub>t Ininv\<^sub>t (\<lambda>_. True) (srb2gsrb (\<lambda> s v. v = b')) ''C2P'') @\<^sub>t P_inv_ind a' b' list) tr 
    \<Longrightarrow> \<exists> tr1 tr2. (Waitinv\<^sub>t (gsb2gsrb(sb2gsb inv)) (\<lambda> d. d = 1) ({}, {}) 
-  @\<^sub>t Waitinv\<^sub>t (gsb2gsrb(sb2gsb inv)) (\<lambda>_. True) ({''P2C''}, {})
-  @\<^sub>t Outinv\<^sub>t (\<lambda>_. True) (srb2gsrb (\<lambda> s v. v = s X)) ''P2C'' 
+  @\<^sub>t WaitOutinv\<^sub>t (gsb2gsrb(sb2gsb inv)) (\<lambda>_. True) (srb2gsrb (\<lambda> s v. v = s X)) ({''P2C''}, {}) ''P2C''
   @\<^sub>t Ininv\<^sub>t (\<lambda>_. True) (srb2gsrb (\<lambda> s v. v = a')) ''C2P'' 
   @\<^sub>t Ininv\<^sub>t (\<lambda>_. True) (srb2gsrb (\<lambda> s v. v = b')) ''C2P'') tr1 \<and> P_inv_ind a' b' list tr2 \<and> tr= tr1@tr2"
     by(auto simp add: join_assn_def)
   have 4:"((Waitinv\<^sub>t (gsb2gsrb(sb2gsb inv)) (\<lambda> d. d = 1) ({}, {}) 
-  @\<^sub>t Waitinv\<^sub>t (gsb2gsrb(sb2gsb inv)) (\<lambda>_. True) ({''P2C''}, {})
-  @\<^sub>t Outinv\<^sub>t (\<lambda>_. True) (srb2gsrb (\<lambda> s v. v = s X)) ''P2C'' 
+  @\<^sub>t WaitOutinv\<^sub>t (gsb2gsrb(sb2gsb inv)) (\<lambda>_. True) (srb2gsrb (\<lambda> s v. v = s X)) ({''P2C''}, {}) ''P2C''
   @\<^sub>t Ininv\<^sub>t (\<lambda>_. True) (srb2gsrb (\<lambda> s v. v = a')) ''C2P'' 
   @\<^sub>t Ininv\<^sub>t (\<lambda>_. True) (srb2gsrb (\<lambda> s v. v = b')) ''C2P'') @\<^sub>t P_inv_ind a' b' list) tr 
    \<Longrightarrow> P_inv_ind a b ((a',b')#list) tr"
     subgoal premises pre
   proof-
     obtain tr1 tr2 where g:"(Waitinv\<^sub>t (gsb2gsrb(sb2gsb inv)) (\<lambda> d. d = 1) ({}, {}) 
-  @\<^sub>t Waitinv\<^sub>t (gsb2gsrb(sb2gsb inv)) (\<lambda>_. True) ({''P2C''}, {})
-  @\<^sub>t Outinv\<^sub>t (\<lambda>_. True) (srb2gsrb (\<lambda> s v. v = s X)) ''P2C'' 
+  @\<^sub>t WaitOutinv\<^sub>t (gsb2gsrb(sb2gsb inv)) (\<lambda>_. True) (srb2gsrb (\<lambda> s v. v = s X)) ({''P2C''}, {}) ''P2C''
   @\<^sub>t Ininv\<^sub>t (\<lambda>_. True) (srb2gsrb (\<lambda> s v. v = a')) ''C2P'' 
   @\<^sub>t Ininv\<^sub>t (\<lambda>_. True) (srb2gsrb (\<lambda> s v. v = b')) ''C2P'') tr1 \<and> P_inv_ind a' b' list tr2 \<and> tr= tr1@tr2"
       using pre 3 by auto
@@ -424,7 +415,7 @@ theorem Valid_post_imp:
   using assms unfolding Valid_def entails_def by blast
 
 lemma P_rep:
-  "\<Turnstile> {\<lambda>s tr. inv s \<and> s A = a \<and> s B = b \<and> s T = 0 \<and> (emp\<^sub>t tr)}
+  "\<Turnstile> {\<lambda>s tr. (inv s \<and> s A = a \<and> s B = b \<and> s T = 0) \<and> (emp\<^sub>t tr)}
     Plant
    {\<lambda>s tr. \<exists>Fc . s A = fst(last((a,b)#Fc)) \<and> s B = snd(last((a,b)#Fc)) \<and> s T = 0 
          \<and> P_inv_ind a b Fc tr \<and> (same_pair (butlast((a,b)#Fc)) \<longrightarrow> inv s)}"
@@ -925,8 +916,7 @@ apply (rule Valid_weaken_pre)
            s B = snd (last ((a, b) # Fc)) \<and>
            ((P_inv_ind a b Fc @\<^sub>t (\<up> (same_pair ((a, b) # Fc)) \<longrightarrow>\<^sub>t
              (Waitinv\<^sub>t (gsb2gsrb (sb2gsb local.inv)) (\<lambda>d. d = 1) ({}, {}) @\<^sub>t
-             Waitinv\<^sub>t (gsb2gsrb(sb2gsb inv)) (\<lambda>_. True) ({''P2C''}, {}) @\<^sub>t
-             out_inv_assn (\<lambda>_. True) (srb2gsrb (\<lambda> s v. v = s X)) ''P2C'')))
+             WaitOutinv\<^sub>t (gsb2gsrb(sb2gsb inv)) (\<lambda>_. True) (srb2gsrb (\<lambda> s v. v = s X)) ({''P2C''}, {}) ''P2C'')))
              t) \<and>
            (same_pair ((a, b) # Fc) \<longrightarrow> local.inv s)"])
    prefer 2
@@ -939,12 +929,14 @@ apply (rule Valid_weaken_pre)
         apply(rule conjI)
         subgoal premises pre 
         proof-
-          have 1:"Outinv\<^sub>t (\<lambda>_. True) (srb2gsrb (\<lambda>s v. v = s X)) ''P2C'' [OutBlock ''P2C'' (s X)]"
-            by(auto simp add: out_inv_assn.simps srb2gsrb.simps)
-          have 2:"Waitinv\<^sub>t (gsb2gsrb (sb2gsb local.inv)) (\<lambda>_. True) ({''P2C''}, {}) []"
-            by(auto simp add: wait_inv_assn.simps)
+          have 1:"WaitOutinv\<^sub>t (gsb2gsrb(sb2gsb inv)) (\<lambda>_. True) (srb2gsrb (\<lambda> s v. v = s X)) ({''P2C''}, {}) ''P2C'' [OutBlock ''P2C'' (s X)]"
+                    if "same_pair [(s A, s B)]"
+            apply(auto simp add: wait_out_inv_assn.simps srb2gsrb.simps gsb2gsrb.simps sb2gsb.simps) 
+            apply(rule exI[where x="State s"])
+            apply auto 
+            using pre that by auto
           show ?thesis 
-            using 1 2 pre(5)
+            using 1  pre(5)
             apply(auto simp add: join_assn_def pure_assn_def imp_assn_def) 
             by blast
         qed
@@ -1044,6 +1036,12 @@ apply (rule Valid_weaken_pre)
         have 19:"Outinv\<^sub>t (\<lambda>_. True) (srb2gsrb (\<lambda>s v. v = s X)) ''P2C''
                    [OutBlock ''P2C'' (p d X)]"
           by(auto simp add:out_inv_assn.simps srb2gsrb.simps)
+        have 20:"WaitOutinv\<^sub>t (gsb2gsrb (sb2gsb local.inv)) (\<lambda>_. True) (srb2gsrb (\<lambda>s v. v = s X)) ({''P2C''}, {}) ''P2C''
+                    [WaitBlk (ereal d) (\<lambda>\<tau>. State (p \<tau>)) ({''P2C''}, {}),OutBlock ''P2C'' (p d X)]" if "same_pair [(p 0 A, p 0 B)]"
+          apply(auto simp add: wait_out_inv_assn.simps gsb2gsrb.simps sb2gsb.simps srb2gsrb.simps inv_def)
+          apply(rule exI[where x= "d"])
+          apply(rule exI[where x= "(\<lambda>\<tau>. State (p \<tau>))"])
+          apply auto using pre 17 that by auto
         show ?thesis
           apply(auto simp add: join_assn_def inv_def)
           subgoal using a3
@@ -1051,8 +1049,8 @@ apply (rule Valid_weaken_pre)
           subgoal using b3
             by (smt atLeastAtMost_iff pre(7))
           subgoal 
-            using 18 19 pre(5) apply(auto simp add: join_assn_def pure_assn_def imp_assn_def)
-            by force
+            using 20 pre(5) apply(auto simp add: join_assn_def pure_assn_def imp_assn_def)
+            by blast
           subgoal using 17 by (smt atLeastAtMost_iff pre(7))
           done
       qed
@@ -1064,12 +1062,14 @@ apply (rule Valid_weaken_pre)
         apply(rule conjI)
         subgoal premises pre 
         proof-
-          have 1:"Outinv\<^sub>t (\<lambda>_. True) (srb2gsrb (\<lambda>s v. v = s X)) ''P2C'' [OutBlock ''P2C'' (s X)]"
-            by(auto simp add: out_inv_assn.simps srb2gsrb.simps)
-          have 2:"Waitinv\<^sub>t (gsb2gsrb (sb2gsb local.inv)) (\<lambda>_. True) ({''P2C''}, {}) []"
-            by(auto simp add: wait_inv_assn.simps)
+          have 1:"WaitOutinv\<^sub>t (gsb2gsrb(sb2gsb inv)) (\<lambda>_. True) (srb2gsrb (\<lambda> s v. v = s X)) ({''P2C''}, {}) ''P2C'' [OutBlock ''P2C'' (s X)]"
+                    if "same_pair ((a, b) # Fc)"
+            apply(auto simp add: wait_out_inv_assn.simps srb2gsrb.simps gsb2gsrb.simps sb2gsb.simps) 
+            apply(rule exI[where x="State s"])
+            apply auto 
+            using pre that  by auto
           show ?thesis 
-            using 1 2 pre(5)
+            using 1  pre(5)
             apply(auto simp add: join_assn_def pure_assn_def imp_assn_def) 
             by blast
         qed
@@ -1169,6 +1169,12 @@ apply (rule Valid_weaken_pre)
         have 19:"Outinv\<^sub>t (\<lambda>_. True) (srb2gsrb (\<lambda>s v. v = s X)) ''P2C''
                    [OutBlock ''P2C'' (p d X)]"
           by(auto simp add:out_inv_assn.simps srb2gsrb.simps)
+        have 20:"WaitOutinv\<^sub>t (gsb2gsrb (sb2gsb local.inv)) (\<lambda>_. True) (srb2gsrb (\<lambda>s v. v = s X)) ({''P2C''}, {}) ''P2C''
+                    [WaitBlk (ereal d) (\<lambda>\<tau>. State (p \<tau>)) ({''P2C''}, {}),OutBlock ''P2C'' (p d X)]" if "same_pair ((a, b) # Fc)"
+          apply(auto simp add: wait_out_inv_assn.simps gsb2gsrb.simps sb2gsb.simps srb2gsrb.simps inv_def)
+          apply(rule exI[where x= "d"])
+          apply(rule exI[where x= "(\<lambda>\<tau>. State (p \<tau>))"])
+          apply auto using pre 17 that by auto
         show ?thesis
           apply(auto simp add: join_assn_def inv_def)
           subgoal using a3
@@ -1176,8 +1182,8 @@ apply (rule Valid_weaken_pre)
           subgoal using b3
             using pre(4) pre(7) by auto
           subgoal 
-            using 18 19 pre(5) apply(auto simp add: join_assn_def pure_assn_def imp_assn_def)
-            by force
+            using 20 pre(5) apply(auto simp add: join_assn_def pure_assn_def imp_assn_def)
+            by blast
           subgoal using 17 by (smt atLeastAtMost_iff pre(7))
           done
       qed
@@ -1202,25 +1208,25 @@ apply (rule Valid_weaken_pre)
         using P_inv_snoc[of a b "[]" "[]" "s A" "s B" "tr1 @ tr2 @ tr3 @ tr4"]
         using P_inv_ind.intros(1)
         by auto
-      subgoal for tr6 tr1 tr5 tr2 tr3 tr4
-      using P_inv_snoc[of a b "[]" "[]" "s A" "s B" "tr1 @ tr2 @ tr3 @ tr4 @ tr5 @ tr6"]
+      subgoal for tr5 tr1 tr4 tr2 tr3 
+      using P_inv_snoc[of a b "[]" "[]" "s A" "s B" "tr1 @ tr2 @ tr3 @ tr4 @ tr5"]
         using P_inv_ind.intros(1)
       by auto
       subgoal for tr4 tr1 tr3 tr2 
        using P_inv_snoc[of a b "[]" tr1 "s A" "s B" "tr2 @ tr3 @ tr4"]
       by auto
-    subgoal for tr6 tr1 tr5 tr2 tr3 tr4
-      apply(subgoal_tac"Ininv\<^sub>t (\<lambda>_. True) (srb2gsrb (\<lambda>sa v. v = s A)) ''C2P'' tr5")
+    subgoal for tr5 tr1 tr4 tr2 tr3 
+      apply(subgoal_tac"Ininv\<^sub>t (\<lambda>_. True) (srb2gsrb (\<lambda>sa v. v = s A)) ''C2P'' tr4")
        prefer 2
       subgoal
         apply(auto simp add: in_assn.simps in_inv_assn.simps srb2gsrb.simps)
         done
-      apply(subgoal_tac"Ininv\<^sub>t (\<lambda>_. True) (srb2gsrb (\<lambda>sa v. v = s B)) ''C2P'' tr6")
+      apply(subgoal_tac"Ininv\<^sub>t (\<lambda>_. True) (srb2gsrb (\<lambda>sa v. v = s B)) ''C2P'' tr5")
        prefer 2
       subgoal
         apply(auto simp add: in_assn.simps in_inv_assn.simps srb2gsrb.simps)
         done
-      using P_inv_snoc[of a b "[]" tr1 "s A" "s B" "tr2 @ tr3 @ tr4 @ tr5 @ tr6"]
+      using P_inv_snoc[of a b "[]" tr1 "s A" "s B" "tr2 @ tr3 @ tr4 @ tr5 "]
       apply(auto simp add: join_assn_def) by blast
     done
   done
@@ -1231,29 +1237,40 @@ apply (rule Valid_weaken_pre)
     subgoal for tr4 tr1 tr3 tr2
       using P_inv_snoc[of a b Fc tr1 "s A" "s B" "tr2 @ tr3 @ tr4"]
       by auto
-    subgoal for tr6 tr1 tr5 tr2 tr3 tr4
-      using P_inv_snoc[of a b Fc tr1 "s A" "s B" "tr2 @ tr3 @ tr4 @ tr5 @ tr6"]
+    subgoal for tr5 tr1 tr4 tr2 tr3 
+      using P_inv_snoc[of a b Fc tr1 "s A" "s B" "tr2 @ tr3 @ tr4 @ tr5 "]
       by auto
     subgoal for tr4 tr1 tr3 tr2
       using P_inv_snoc[of a b Fc tr1 "s A" "s B" "tr2 @ tr3 @ tr4"]
       by auto
-    subgoal for tr6 tr1 tr5 tr2 tr3 tr4
-      apply(subgoal_tac"Ininv\<^sub>t (\<lambda>_. True) (srb2gsrb (\<lambda>sa v. v = s A)) ''C2P'' tr5")
+    subgoal for tr5 tr1 tr4 tr2 tr3 
+      apply(subgoal_tac"Ininv\<^sub>t (\<lambda>_. True) (srb2gsrb (\<lambda>sa v. v = s A)) ''C2P'' tr4")
        prefer 2
       subgoal
         apply(auto simp add: in_assn.simps in_inv_assn.simps srb2gsrb.simps)
         done
-      apply(subgoal_tac"Ininv\<^sub>t (\<lambda>_. True) (srb2gsrb (\<lambda>sa v. v = s B)) ''C2P'' tr6")
+      apply(subgoal_tac"Ininv\<^sub>t (\<lambda>_. True) (srb2gsrb (\<lambda>sa v. v = s B)) ''C2P'' tr5")
        prefer 2
       subgoal
         apply(auto simp add: in_assn.simps in_inv_assn.simps srb2gsrb.simps)
         done
-      using P_inv_snoc[of a b Fc tr1 "s A" "s B" "tr2 @ tr3 @ tr4 @ tr5 @ tr6"]
+      using P_inv_snoc[of a b Fc tr1 "s A" "s B" "tr2 @ tr3 @ tr4 @ tr5 "]
       apply(auto simp add:join_assn_def) by blast
     done
   done
   done
   done
+
+lemma P_rep':
+  "\<Turnstile> {\<lambda>s tr. (inv s \<and> s A = a \<and> s B = b \<and> s T = 0) \<and> (emp\<^sub>t tr)}
+    Plant
+   {\<lambda>s tr. \<exists>Fc . (s A = fst(last((a,b)#Fc)) \<and> s B = snd(last((a,b)#Fc)) \<and> s T = 0) 
+         \<and> P_inv_ind a b Fc tr }"
+  apply(rule Valid_strengthen_post)
+   prefer 2
+   apply(rule P_rep)
+  by(auto simp add: entails_def)
+
 
 inductive tot_block :: "real list  \<Rightarrow> tassn" where
   "tot_block  [] []"
@@ -1265,6 +1282,59 @@ inductive tot_block :: "real list  \<Rightarrow> tassn" where
    tot_block fc tr2 \<Longrightarrow>
    tot_block (x#fc) (tr1@tr2)"
 
+lemma tot_block_prop1:
+"tot_block (x#list) = Waitinv\<^sub>t (pgsrb2gsrb (gsb2gsrb(sb2gsb inv)) (\<lambda>_ _ . True))(\<lambda> d. d = 1) ({}, {})  @\<^sub>t
+   Waitinv\<^sub>t (pgsrb2gsrb (gsb2gsrb(sb2gsb inv)) (\<lambda>_ _ . True))(\<lambda> d. True) ({''P2C''}, {})  @\<^sub>t
+   IOinv\<^sub>t (\<lambda> _. True)(\<lambda> s v. v = x)''P2C''  @\<^sub>t
+   IOinv\<^sub>t (\<lambda> _. True)(\<lambda> s v. v = p x)''C2P'' @\<^sub>t
+   IOinv\<^sub>t (\<lambda> _. True)(\<lambda> s v. v = p x)''C2P'' @\<^sub>t tot_block list"
+apply(rule ext)
+  subgoal for tr
+proof-
+  have 1:"tot_block (x#list) tr \<Longrightarrow> \<exists> tr1 tr2. (Waitinv\<^sub>t (pgsrb2gsrb (gsb2gsrb(sb2gsb inv)) (\<lambda>_ _ . True))(\<lambda> d. d = 1) ({}, {})  @\<^sub>t
+   Waitinv\<^sub>t (pgsrb2gsrb (gsb2gsrb(sb2gsb inv)) (\<lambda>_ _ . True))(\<lambda> d. True) ({''P2C''}, {})  @\<^sub>t
+   IOinv\<^sub>t (\<lambda> _. True)(\<lambda> s v. v = x)''P2C''  @\<^sub>t
+   IOinv\<^sub>t (\<lambda> _. True)(\<lambda> s v. v = p x)''C2P'' @\<^sub>t
+   IOinv\<^sub>t (\<lambda> _. True)(\<lambda> s v. v = p x)''C2P'') tr1 \<and> tot_block list tr2 \<and> tr=tr1@tr2"
+    apply(rule tot_block.cases[of "(x # list)" tr]) 
+    by auto
+  have 2:"tot_block (x#list) tr \<Longrightarrow> ((Waitinv\<^sub>t (pgsrb2gsrb (gsb2gsrb(sb2gsb inv)) (\<lambda>_ _ . True))(\<lambda> d. d = 1) ({}, {})  @\<^sub>t
+   Waitinv\<^sub>t (pgsrb2gsrb (gsb2gsrb(sb2gsb inv)) (\<lambda>_ _ . True))(\<lambda> d. True) ({''P2C''}, {})  @\<^sub>t
+   IOinv\<^sub>t (\<lambda> _. True)(\<lambda> s v. v = x)''P2C''  @\<^sub>t
+   IOinv\<^sub>t (\<lambda> _. True)(\<lambda> s v. v = p x)''C2P'' @\<^sub>t
+   IOinv\<^sub>t (\<lambda> _. True)(\<lambda> s v. v = p x)''C2P'') @\<^sub>t tot_block list ) tr"
+    using 1 join_assn_def by auto
+  have 3:"((Waitinv\<^sub>t (pgsrb2gsrb (gsb2gsrb(sb2gsb inv)) (\<lambda>_ _ . True))(\<lambda> d. d = 1) ({}, {})  @\<^sub>t
+   Waitinv\<^sub>t (pgsrb2gsrb (gsb2gsrb(sb2gsb inv)) (\<lambda>_ _ . True))(\<lambda> d. True) ({''P2C''}, {})  @\<^sub>t
+   IOinv\<^sub>t (\<lambda> _. True)(\<lambda> s v. v = x)''P2C''  @\<^sub>t
+   IOinv\<^sub>t (\<lambda> _. True)(\<lambda> s v. v = p x)''C2P'' @\<^sub>t
+   IOinv\<^sub>t (\<lambda> _. True)(\<lambda> s v. v = p x)''C2P'') @\<^sub>t tot_block list ) tr \<Longrightarrow>
+    \<exists> tr1 tr2. (Waitinv\<^sub>t (pgsrb2gsrb (gsb2gsrb(sb2gsb inv)) (\<lambda>_ _ . True))(\<lambda> d. d = 1) ({}, {})  @\<^sub>t
+   Waitinv\<^sub>t (pgsrb2gsrb (gsb2gsrb(sb2gsb inv)) (\<lambda>_ _ . True))(\<lambda> d. True) ({''P2C''}, {})  @\<^sub>t
+   IOinv\<^sub>t (\<lambda> _. True)(\<lambda> s v. v = x)''P2C''  @\<^sub>t
+   IOinv\<^sub>t (\<lambda> _. True)(\<lambda> s v. v = p x)''C2P'' @\<^sub>t
+   IOinv\<^sub>t (\<lambda> _. True)(\<lambda> s v. v = p x)''C2P'') tr1 \<and> tot_block list tr2 \<and> tr=tr1@tr2"
+    by(auto simp add: join_assn_def)
+  have 4:"((Waitinv\<^sub>t (pgsrb2gsrb (gsb2gsrb(sb2gsb inv)) (\<lambda>_ _ . True))(\<lambda> d. d = 1) ({}, {})  @\<^sub>t
+   Waitinv\<^sub>t (pgsrb2gsrb (gsb2gsrb(sb2gsb inv)) (\<lambda>_ _ . True))(\<lambda> d. True) ({''P2C''}, {})  @\<^sub>t
+   IOinv\<^sub>t (\<lambda> _. True)(\<lambda> s v. v = x)''P2C''  @\<^sub>t
+   IOinv\<^sub>t (\<lambda> _. True)(\<lambda> s v. v = p x)''C2P'' @\<^sub>t
+   IOinv\<^sub>t (\<lambda> _. True)(\<lambda> s v. v = p x)''C2P'') @\<^sub>t tot_block list ) tr \<Longrightarrow> tot_block (x#list) tr"
+    subgoal premises pre
+    proof-
+      obtain tr1 tr2 where g:"(Waitinv\<^sub>t (pgsrb2gsrb (gsb2gsrb(sb2gsb inv)) (\<lambda>_ _ . True))(\<lambda> d. d = 1) ({}, {})  @\<^sub>t
+   Waitinv\<^sub>t (pgsrb2gsrb (gsb2gsrb(sb2gsb inv)) (\<lambda>_ _ . True))(\<lambda> d. True) ({''P2C''}, {})  @\<^sub>t
+   IOinv\<^sub>t (\<lambda> _. True)(\<lambda> s v. v = x)''P2C''  @\<^sub>t
+   IOinv\<^sub>t (\<lambda> _. True)(\<lambda> s v. v = p x)''C2P'' @\<^sub>t
+   IOinv\<^sub>t (\<lambda> _. True)(\<lambda> s v. v = p x)''C2P'') tr1" "tot_block list tr2" "tr=tr1@tr2"
+        using pre 3 by auto
+      then show ?thesis
+        using tot_block.intros(2)[of x tr1 list tr2] by auto
+    qed
+  done
+    then show ?thesis using 2 4 by(auto simp add: join_assoc)
+  qed
+  done
 lemma g1:
  "combine_assn chs
      (Waitinv\<^sub>t r (\<lambda>d. d = 1) ({}, {}) @\<^sub>t P)
@@ -1324,11 +1394,121 @@ qed
 lemma g2:
   assumes "ch \<in> chs"
   shows "combine_assn chs
-     (Waitinv\<^sub>t r (\<lambda>d. True) ({ch}, {}) @\<^sub>t Outinv\<^sub>t (\<lambda>_. True) (srb2gsrb (\<lambda> s v. v = s X)) ch @\<^sub>t P)
-     (Waitinv\<^sub>t (\<lambda>_ _. True) (\<lambda> d. d > 0) ({}, {}) @\<^sub>t Ininv\<^sub>t (\<lambda>_. True) (srb2gsrb (\<lambda> s v. v = x)) ch @\<^sub>t Q) 
+     (WaitOutinv\<^sub>t (gsb2gsrb (sb2gsb local.inv)) (\<lambda>_. True) (srb2gsrb (\<lambda>s v. v = s X)) ({ch}, {}) ch  @\<^sub>t P)
+     (Waitinv\<^sub>t (\<lambda>_ _. True) (\<lambda> d. d > 0) ({}, {}) @\<^sub>t Q) 
       \<Longrightarrow>\<^sub>t 
-   (Waitinv\<^sub>t (pgsrb2gsrb r (\<lambda>_ _ . True))(\<lambda>_. True) ({ch}, {}) 
-      @\<^sub>t IOinv\<^sub>t (\<lambda> _. True)(\<lambda> s v. v = x) ch  @\<^sub>t combine_assn chs P Q )"
+   (Waitinv\<^sub>t (pgsrb2gsrb (gsb2gsrb (sb2gsb local.inv)) (\<lambda>_ _ . True))(\<lambda>_. True) ({ch}, {}) 
+     @\<^sub>t combine_assn chs (WaitOutinv\<^sub>t (gsb2gsrb (sb2gsb local.inv)) (\<lambda>_. True) (srb2gsrb (\<lambda>s v. v = s X)) ({ch}, {}) ch  @\<^sub>t P)  Q )"
+proof-
+  have * :"(Waitinv\<^sub>t (pgsrb2gsrb (gsb2gsrb (sb2gsb local.inv)) (\<lambda>_ _ . True))(\<lambda>_. True) ({ch}, {}) 
+     @\<^sub>t combine_assn chs (WaitOutinv\<^sub>t (gsb2gsrb (sb2gsb local.inv)) (\<lambda>_. True) (srb2gsrb (\<lambda>s v. v = s X)) ({ch}, {}) ch  @\<^sub>t P)  Q ) tr"
+    if "(WaitOutinv\<^sub>t (gsb2gsrb (sb2gsb local.inv)) (\<lambda>_. True) (srb2gsrb (\<lambda>s v. v = s X)) ({ch}, {}) ch  @\<^sub>t P) tr1"
+       "(Waitinv\<^sub>t (\<lambda>_ _. True) (\<lambda> d. d > 0) ({}, {})  @\<^sub>t Q) tr2"
+       "combine_blocks chs tr1 tr2 tr" for tr tr1 tr2
+proof -
+    from that(1)[unfolded join_assn_def]
+    obtain tr11 tr12 where a: "WaitOutinv\<^sub>t (gsb2gsrb (sb2gsb local.inv)) (\<lambda>_. True) (srb2gsrb (\<lambda>s v. v = s X)) ({ch}, {}) ch  tr11" "P tr12" "tr1 = tr11 @ tr12"
+      by auto
+    from that(2)[unfolded join_assn_def]
+    obtain tr21 tr22 where b: "Waitinv\<^sub>t (\<lambda>_ _. True) (\<lambda> d. d > 0) ({}, {}) tr21" "Q tr22" "tr2 = tr21 @ tr22"
+      by auto
+    have g:"(Waitinv\<^sub>t (pgsrb2gsrb (gsb2gsrb (sb2gsb local.inv)) (\<lambda>_ _. True)) (\<lambda>_. True) ({ch}, {}) @\<^sub>t
+     combine_assn chs (WaitOutinv\<^sub>t (gsb2gsrb (sb2gsb local.inv)) (\<lambda>_. True) (srb2gsrb (\<lambda>s v. v = s X)) ({ch}, {}) ch @\<^sub>t P) Q)
+     tr" if "combine_blocks chs (WaitBlk (ereal d) p ({ch}, {}) # OutBlock ch v # tr12) (WaitBlk (ereal d') p' ({}, {}) # tr22) tr" 
+      "d>0" "d'>0" "\<forall>t\<in>{0..d}. gsb2gsrb (sb2gsb local.inv) (p t) t" "srb2gsrb (\<lambda>s v. v = s X) (p d) v"for v d p d' p'
+    proof -
+      have "d < d' \<or> d = d' \<or> d > d'" by auto
+      then show ?thesis
+      proof (elim disjE)
+        assume d1: "d < d'"
+        have d1': "ereal d < ereal d'"
+          using d1 by auto
+        show ?thesis
+          using that
+          apply (elim combine_blocks_waitE3) apply (rule that(2))
+            apply (rule d1') apply auto
+          using assms(1) combine_blocks_pairE2 by blast
+      next
+        assume d2: "d = d'"
+        show ?thesis
+          using that(1)
+          unfolding d2[symmetric]
+          apply (elim combine_blocks_waitE2)
+          apply auto
+          subgoal for blks'
+            apply (subst join_assn_def)
+            apply (rule exI[where x="[WaitBlk (ereal d) (\<lambda>t. ParState (p t) (p' t)) ({ch}, {})]"])
+            apply (rule exI[where x=blks'])
+            apply (rule conjI)
+            subgoal using d2 that using wait_inv_assn.intros(2)[of d "(\<lambda>_. True)" "(pgsrb2gsrb (gsb2gsrb (sb2gsb local.inv)) (\<lambda>_ _. True))" "(\<lambda>t. ParState (p t) (p' t))" "({ch}, {})"]
+              by(auto simp add:pgsrb2gsrb.simps)
+            apply (rule conjI)
+             prefer 2 subgoal by auto
+            unfolding combine_assn_def
+            apply (rule exI[where x="(OutBlock ch v # tr12)"])
+            apply (rule exI[where x=tr22])
+            apply (rule conjI)
+             prefer 2 subgoal using b(2) by auto
+            unfolding join_assn_def
+            apply (rule exI[where x="[OutBlock ch v]"])
+            apply (rule exI[where x=tr12])
+            using that(2,4,5)
+            by (auto simp add: a(2) wait_out_inv_assn.simps gsb2gsrb.simps)
+          done
+      next
+        assume d3: "d > d'"
+        have d3': "ereal d > ereal d'"
+          using d3 by auto
+        show ?thesis
+          using that(1)
+          apply (elim combine_blocks_waitE4) apply (rule that(3))
+            apply (rule d3') apply auto
+          subgoal for blks'
+            unfolding pure_assn_def conj_assn_def
+            apply (subst join_assn_def)
+            apply (rule exI[where x="[WaitBlk (ereal d') (\<lambda>t. ParState (p t) (p' t)) ({ch}, {})]"])
+            apply (rule exI[where x=blks'])
+            apply (rule conjI)
+            subgoal using wait_inv_assn.intros(2)[of d' "(\<lambda>_. True)" "(pgsrb2gsrb (gsb2gsrb (sb2gsb local.inv)) (\<lambda>_ _. True))" " (\<lambda>t. ParState (p t) (p' t))" "({ch}, {})"]
+              using that(3,4,5) d3 by(auto simp add:pgsrb2gsrb.simps)
+            apply (rule conjI)
+             prefer 2 subgoal by auto
+            unfolding combine_assn_def
+            apply (rule exI[where x="WaitBlk (ereal (d - d')) (\<lambda>t. p (t + d')) ({ch}, {}) # OutBlock ch v # tr12"])
+            apply (rule exI[where x=tr22])
+            apply (rule conjI)
+             prefer 2 subgoal apply (rule conjI)
+               apply (rule b(2)) by auto
+            unfolding join_assn_def
+            apply (rule exI[where x="[WaitBlk (ereal (d - d')) (\<lambda>t. p (t + d')) ({ch}, {}), OutBlock ch v]"])
+            apply (rule exI[where x=tr12])
+            apply (rule conjI)
+            subgoal
+              using that d3
+              using wait_out_inv_assn.intros(2)[of "d-d'" "(\<lambda>_. True)" "(gsb2gsrb (sb2gsb local.inv))" "(\<lambda>t. p (t + d'))" "(srb2gsrb (\<lambda>s v. v = s X))" "v" "({ch}, {})" ch]
+               by(auto simp add:gsb2gsrb.simps)
+            using a(2) by auto
+          done
+      qed
+    qed
+    show ?thesis
+      using a(1) apply (cases rule: wait_out_inv_assn.cases)
+      using b(1) apply (cases rule: wait_inv_assn.cases)
+        apply auto
+      subgoal for v d p s
+        using that a b apply auto
+        using assms combine_blocks_pairE2 by blast
+      using b(1) apply (cases rule: wait_inv_assn.cases)
+       apply auto
+      subgoal for d p v d' p'
+        using g[of d p v d' p'] that a b by auto
+      done
+  qed
+  then show ?thesis
+    apply (subst combine_assn_def)
+    by (auto simp add: entails_tassn_def)
+qed
+        
 
 
 
@@ -1358,9 +1538,17 @@ next
     by auto
 qed
 
+lemma entails_tassn_cancel_both_m:
+  assumes "P \<Longrightarrow>\<^sub>t Q"
+    and "\<forall>tr. P tr \<longrightarrow> f"
+    and "f \<Longrightarrow> R \<Longrightarrow>\<^sub>t S"
+  shows "P @\<^sub>t R \<Longrightarrow>\<^sub>t Q @\<^sub>t S"
+  using assms
+  by (auto simp add: entails_tassn_def join_assn_def)
+ 
 
 lemma combine:
- "combine_assn {''P2C'', ''C2P''} (P_inv_ind a a ps) (C_inv_ind cs) \<Longrightarrow>\<^sub>t  tot_block cs \<and>\<^sub>t \<up>(same_pair ((a,a)#ps))"
+ "combine_assn {''P2C'', ''C2P''} (P_inv_ind a a ps) (C_inv_ind cs) \<Longrightarrow>\<^sub>t  tot_block cs"
 proof(induction ps arbitrary: cs a)
 case Nil
   then show ?case 
@@ -1400,35 +1588,95 @@ case Nil
   qed
 
 next
-  case (Cons p ps)
+  case (Cons pp ps)
   note Cons1 = Cons
   then show ?case 
   proof (cases cs)
       case Nil
       then show ?thesis
-        apply(cases p)
+        apply(cases pp)
         apply(auto simp add:C_inv_prop0 P_inv_prop1 same_pair.intros)
         subgoal for a' b'
           apply (rule entails_tassn_trans)
            apply (subst combine_assn_waitinv_emp)
            apply auto
       apply (rule entails_tassn_trans)
-           apply (subst combine_assn_waitinv_emp)
+           apply (subst combine_assn_waitoutinv_emp)
            apply auto
-      apply (rule entails_tassn_trans)
-           apply (subst combine_assn_outinv_emp)
-            apply auto
-          by (rule false_assn_entails)
+          done
         done
     next
       case (Cons c list)
       then show ?thesis
-        apply (cases p)
+        apply (cases pp)
         subgoal for a' b'
-          apply(auto simp add:P_inv_prop1 C_inv_prop1)
-      qed
+         apply(auto simp add:P_inv_prop1 C_inv_prop1 tot_block_prop1 )
+          apply (rule entails_tassn_trans)
+           apply(subst g1)
+           apply auto
+          apply (rule entails_tassn_cancel_left)
+          apply (rule entails_tassn_trans)
+           apply(subst g2)
+            apply auto
+          apply (rule entails_tassn_cancel_left)
+          apply (rule entails_tassn_trans)
+           apply(subst combine_assn_waitoutinv_ininv)
+             apply auto
+          apply (rule entails_tassn_cancel_both)
+          subgoal by(auto simp add:entails_tassn_def io_inv_assn.simps pgsb2gsb.simps pgsrb2gsrb.simps srb2gsrb.simps)
+          apply (rule entails_tassn_trans)
+           apply(subst combine_assn_ininv_outinv)
+            apply auto
+          apply (rule entails_tassn_cancel_both_m[where f="a' = p c"])
+          subgoal by(auto simp add:entails_tassn_def io_inv_assn.simps pgsb2gsb.simps pgsrb2gsrb.simps srb2gsrb.simps)
+          subgoal by(auto simp add:entails_tassn_def io_inv_assn.simps pgsb2gsb.simps pgsrb2gsrb.simps srb2gsrb.simps)
+          apply (rule entails_tassn_trans)
+           apply(subst combine_assn_ininv_outinv)
+            apply auto
+          apply (rule entails_tassn_cancel_both_m[where f="b' = p c"])
+          subgoal by(auto simp add:entails_tassn_def io_inv_assn.simps pgsb2gsb.simps pgsrb2gsrb.simps srb2gsrb.simps)
+          subgoal by(auto simp add:entails_tassn_def io_inv_assn.simps pgsb2gsb.simps pgsrb2gsrb.simps srb2gsrb.simps)
+          apply auto
+          using Cons1
+          by auto
+        done
+    qed
+  qed
 
-qed
 
+lemma sing_gassn_split_m3:
+  "sing_gassn (\<lambda>s tr. P1 s \<and> P2 s \<and> P3 s \<and> Q tr) = (state_gassn (sing_assn (\<lambda> s. P1 s \<and> P2 s \<and> P3 s)) \<and>\<^sub>g trace_gassn Q)"
+  apply (rule ext) apply (rule ext)
+  subgoal for s tr
+    apply (cases s) by (auto simp add: state_gassn_def trace_gassn_def and_gassn_def)
+  done
+
+
+lemma system_Prop:
+ "\<Turnstile>\<^sub>p {pair_assn (\<lambda>s. inv s \<and> s A = a \<and> s B = a \<and> s T = 0 )
+               (\<lambda>s. s X = x)}
+      Parallel (Single Plant)
+                     {''P2C'', ''C2P''}
+                     (Single Control)
+    {\<exists>\<^sub>g cs. trace_gassn (tot_block cs)}"
+  apply (rule ParValid_conseq')
+    apply (rule ParValid_Parallel')
+     apply(rule P_rep')
+    apply(rule C_rep)
+   apply (auto simp add: sing_gassn_split sing_gassn_ex sing_gassn_split_m3)
+    apply (rule sync_gassn_ex_pre_left)
+  apply (rule sync_gassn_ex_pre_right)
+  subgoal for ps cs
+unfolding sync_gassn_state_left sync_gassn_state_right
+  apply (rule entails_ex_gassn)
+  apply(rule exI[where x="cs"])
+  apply (rule and_entails_gassn2[OF sync_gassn_traces])
+    apply (rule and_entails_gassn2[OF entails_trace_gassn])
+     apply (rule entails_tassn_trans)
+      prefer 2 apply(rule combine)
+  apply (rule combine_assn_mono)
+  apply (auto simp add: entails_tassn_def entails_gassn_def and_gassn_def)
+  done
+  done
 end
 end
